<?xml version="1.0"?>
<rdf:RDF xmlns="http://www.semanticweb.org/alber/ontologies/2020/10/untitled-ontology-5#"
     xml:base="http://www.semanticweb.org/alber/ontologies/2020/10/untitled-ontology-5"
     xmlns:owl="http://www.w3.org/2002/07/owl#"
     xmlns:rdf="http://www.w3.org/1999/02/22-rdf-syntax-ns#"
     xmlns:xml="http://www.w3.org/XML/1998/namespace"
     xmlns:xsd="http://www.w3.org/2001/XMLSchema#"
     xmlns:cube="http://purl.org/linked-data/cube#"
     xmlns:rdfs="http://www.w3.org/2000/01/rdf-schema#"
     xmlns:skos="http://www.w3.org/2004/02/skos/core#"
     xmlns:time="http://www.w3.org/2006/time#"
     xmlns:ontological-engineering-project="http://www.semanticweb.org/alber/ontologies/2020/10/ontological-engineering-project#">
    <owl:Ontology rdf:about="http://www.semanticweb.org/alber/ontologies/2020/10/ontological-engineering-project"/>
    


    <!-- 
    ///////////////////////////////////////////////////////////////////////////////////////
    //
    // Annotation properties
    //
    ///////////////////////////////////////////////////////////////////////////////////////
     -->

    


    <!-- http://www.w3.org/2004/02/skos/core#definition -->

    <owl:AnnotationProperty rdf:about="http://www.w3.org/2004/02/skos/core#definition"/>
    


    <!-- http://www.w3.org/2004/02/skos/core#note -->

    <owl:AnnotationProperty rdf:about="http://www.w3.org/2004/02/skos/core#note"/>
    


    <!-- 
    ///////////////////////////////////////////////////////////////////////////////////////
    //
    // Object Properties
    //
    ///////////////////////////////////////////////////////////////////////////////////////
     -->

    


    <!-- http://purl.org/linked-data/cube#dataSet -->

    <owl:ObjectProperty rdf:about="http://purl.org/linked-data/cube#dataSet">
        <rdfs:domain rdf:resource="http://purl.org/linked-data/cube#Observation"/>
        <rdfs:range rdf:resource="http://purl.org/linked-data/cube#DataSet"/>
        <rdfs:comment xml:lang="en">indicates the data set of which this observation is a part</rdfs:comment>
        <rdfs:isDefinedBy rdf:resource="http://purl.org/linked-data/cube"/>
        <rdfs:label xml:lang="en">data set</rdfs:label>
    </owl:ObjectProperty>
    


    <!-- http://www.semanticweb.org/alber/ontologies/2020/10/ontological-engineering-project#deVisita -->

    <owl:ObjectProperty rdf:about="http://www.semanticweb.org/alber/ontologies/2020/10/ontological-engineering-project#deVisita">
        <owl:inverseOf rdf:resource="http://www.semanticweb.org/alber/ontologies/2020/10/ontological-engineering-project#enIntervaloDeTiempo"/>
        <rdfs:domain rdf:resource="http://www.w3.org/2006/time#DateTimeInterval"/>
        <rdfs:range rdf:resource="http://www.semanticweb.org/alber/ontologies/2020/10/untitled-ontology-5#Visita"/>
        <rdfs:label xml:lang="es">deVisita</rdfs:label>
        <rdfs:label xml:lang="en">ofVisit</rdfs:label>
    </owl:ObjectProperty>
    


    <!-- http://www.semanticweb.org/alber/ontologies/2020/10/ontological-engineering-project#enIntervaloDeTiempo -->

    <owl:ObjectProperty rdf:about="http://www.semanticweb.org/alber/ontologies/2020/10/ontological-engineering-project#enIntervaloDeTiempo">
        <rdfs:domain rdf:resource="http://www.semanticweb.org/alber/ontologies/2020/10/untitled-ontology-5#Visita"/>
        <rdfs:range rdf:resource="http://www.w3.org/2006/time#DateTimeInterval"/>
        <rdfs:label xml:lang="es">enIntervaloDeTiempo</rdfs:label>
        <rdfs:label xml:lang="en">inTimeInterval</rdfs:label>
    </owl:ObjectProperty>
    


    <!-- http://www.semanticweb.org/alber/ontologies/2020/10/ontological-engineering-project#esEquipamientoDe -->

    <owl:ObjectProperty rdf:about="http://www.semanticweb.org/alber/ontologies/2020/10/ontological-engineering-project#esEquipamientoDe">
        <owl:inverseOf rdf:resource="http://www.semanticweb.org/alber/ontologies/2020/10/ontological-engineering-project#tieneEquipamiento"/>
        <rdfs:domain rdf:resource="http://www.semanticweb.org/alber/ontologies/2020/10/untitled-ontology-5#Equipamiento"/>
        <rdfs:range rdf:resource="http://www.semanticweb.org/alber/ontologies/2020/10/untitled-ontology-5#Espacio_Natural"/>
        <rdfs:label xml:lang="es">esEquipamientoDe</rdfs:label>
        <rdfs:label xml:lang="en">isEquipmentOf</rdfs:label>
    </owl:ObjectProperty>
    


    <!-- http://www.semanticweb.org/alber/ontologies/2020/10/ontological-engineering-project#esEspacioNaturalDe -->

    <owl:ObjectProperty rdf:about="http://www.semanticweb.org/alber/ontologies/2020/10/ontological-engineering-project#esEspacioNaturalDe">
        <owl:inverseOf rdf:resource="http://www.semanticweb.org/alber/ontologies/2020/10/ontological-engineering-project#tieneEspacioNatural"/>
        <rdfs:domain rdf:resource="http://www.semanticweb.org/alber/ontologies/2020/10/untitled-ontology-5#Espacio_Natural"/>
        <rdfs:range rdf:resource="http://www.semanticweb.org/alber/ontologies/2020/10/untitled-ontology-5#Provincia"/>
        <rdfs:label xml:lang="es">esEspacioNaturalDe</rdfs:label>
        <rdfs:label xml:lang="en">isNaturalSpaceOf</rdfs:label>
    </owl:ObjectProperty>
    


    <!-- http://www.semanticweb.org/alber/ontologies/2020/10/ontological-engineering-project#esParteDe -->

    <owl:ObjectProperty rdf:about="http://www.semanticweb.org/alber/ontologies/2020/10/ontological-engineering-project#esParteDe">
        <owl:inverseOf rdf:resource="http://www.semanticweb.org/alber/ontologies/2020/10/ontological-engineering-project#tieneParte"/>
        <rdfs:label xml:lang="es">esParteDe</rdfs:label>
        <rdfs:label xml:lang="en">isPartOf</rdfs:label>
    </owl:ObjectProperty>
    


    <!-- http://www.semanticweb.org/alber/ontologies/2020/10/ontological-engineering-project#tieneEquipamiento -->

    <owl:ObjectProperty rdf:about="http://www.semanticweb.org/alber/ontologies/2020/10/ontological-engineering-project#tieneEquipamiento">
        <rdfs:domain rdf:resource="http://www.semanticweb.org/alber/ontologies/2020/10/untitled-ontology-5#Espacio_Natural"/>
        <rdfs:range rdf:resource="http://www.semanticweb.org/alber/ontologies/2020/10/untitled-ontology-5#Equipamiento"/>
        <rdfs:label xml:lang="en">hasEquipment</rdfs:label>
        <rdfs:label xml:lang="es">tieneEquipamiento</rdfs:label>
    </owl:ObjectProperty>
    


    <!-- http://www.semanticweb.org/alber/ontologies/2020/10/ontological-engineering-project#tieneEspacioNatural -->

    <owl:ObjectProperty rdf:about="http://www.semanticweb.org/alber/ontologies/2020/10/ontological-engineering-project#tieneEspacioNatural">
        <rdfs:domain rdf:resource="http://www.semanticweb.org/alber/ontologies/2020/10/untitled-ontology-5#Provincia"/>
        <rdfs:range rdf:resource="http://www.semanticweb.org/alber/ontologies/2020/10/untitled-ontology-5#Espacio_Natural"/>
        <rdfs:label xml:lang="en">hasNaturalSpace</rdfs:label>
        <rdfs:label xml:lang="es">tieneEspacioNatural</rdfs:label>
    </owl:ObjectProperty>
    


    <!-- http://www.semanticweb.org/alber/ontologies/2020/10/ontological-engineering-project#tieneParte -->

    <owl:ObjectProperty rdf:about="http://www.semanticweb.org/alber/ontologies/2020/10/ontological-engineering-project#tieneParte">
        <rdfs:label xml:lang="en">hasPart</rdfs:label>
        <rdfs:label xml:lang="es">tieneParte</rdfs:label>
    </owl:ObjectProperty>
    


    <!-- http://www.semanticweb.org/alber/ontologies/2020/10/ontological-engineering-project#tieneProcedencia -->

    <owl:ObjectProperty rdf:about="http://www.semanticweb.org/alber/ontologies/2020/10/ontological-engineering-project#tieneProcedencia">
        <rdfs:domain rdf:resource="http://www.semanticweb.org/alber/ontologies/2020/10/untitled-ontology-5#Visita"/>
        <rdfs:range rdf:resource="http://www.semanticweb.org/alber/ontologies/2020/10/untitled-ontology-5#Lugar_Procedencia"/>
        <rdfs:label xml:lang="en">hasOrigin</rdfs:label>
        <rdfs:label xml:lang="es">tieneProcedencia</rdfs:label>
    </owl:ObjectProperty>
    


    <!-- http://www.semanticweb.org/alber/ontologies/2020/10/ontological-engineering-project#tieneVisita -->

    <owl:ObjectProperty rdf:about="http://www.semanticweb.org/alber/ontologies/2020/10/ontological-engineering-project#tieneVisita">
        <owl:inverseOf rdf:resource="http://www.semanticweb.org/alber/ontologies/2020/10/ontological-engineering-project#visitaAlEquipamiento"/>
        <rdfs:domain rdf:resource="http://www.semanticweb.org/alber/ontologies/2020/10/untitled-ontology-5#Equipamiento"/>
        <rdfs:range rdf:resource="http://www.semanticweb.org/alber/ontologies/2020/10/untitled-ontology-5#Visita"/>
        <rdfs:label xml:lang="en">hasVisit</rdfs:label>
        <rdfs:label xml:lang="es">tieneVisita</rdfs:label>
    </owl:ObjectProperty>
    


    <!-- http://www.semanticweb.org/alber/ontologies/2020/10/ontological-engineering-project#visitaAlEquipamiento -->

    <owl:ObjectProperty rdf:about="http://www.semanticweb.org/alber/ontologies/2020/10/ontological-engineering-project#visitaAlEquipamiento">
        <rdfs:domain rdf:resource="http://www.semanticweb.org/alber/ontologies/2020/10/untitled-ontology-5#Visita"/>
        <rdfs:range rdf:resource="http://www.semanticweb.org/alber/ontologies/2020/10/untitled-ontology-5#Equipamiento"/>
        <rdfs:label xml:lang="es">visitaAlEquipamiento</rdfs:label>
    </owl:ObjectProperty>
    


    <!-- http://www.w3.org/2006/time#hasDateTimeDescription -->

    <owl:ObjectProperty rdf:about="http://www.w3.org/2006/time#hasDateTimeDescription">
        <rdfs:domain rdf:resource="http://www.w3.org/2006/time#DateTimeInterval"/>
        <rdfs:range rdf:resource="http://www.w3.org/2006/time#GeneralDateTimeDescription"/>
        <rdfs:comment xml:lang="es">Valor de intervalo de fecha-hora expresado como un valor estructurado. El principio y el final del intervalo coincide con los límites del elemento más corto en la descripción.</rdfs:comment>
        <rdfs:comment xml:lang="en">Value of DateTimeInterval expressed as a structured value. The beginning and end of the interval coincide with the limits of the shortest element in the description.</rdfs:comment>
        <rdfs:label xml:lang="en">has Date-Time description</rdfs:label>
        <rdfs:label xml:lang="es">tiene descripción fecha-hora</rdfs:label>
        <skos:definition xml:lang="es">Valor de intervalo de fecha-hora expresado como un valor estructurado. El principio y el final del intervalo coincide con los límites del elemento más corto en la descripción.</skos:definition>
        <skos:definition xml:lang="en">Value of DateTimeInterval expressed as a structured value. The beginning and end of the interval coincide with the limits of the shortest element in the description.</skos:definition>
    </owl:ObjectProperty>
    


    <!-- 
    ///////////////////////////////////////////////////////////////////////////////////////
    //
    // Data properties
    //
    ///////////////////////////////////////////////////////////////////////////////////////
     -->

    


    <!-- http://www.semanticweb.org/alber/ontologies/2020/10/ontological-engineering-project#numero_de_visitantes -->

    <owl:DatatypeProperty rdf:about="http://www.semanticweb.org/alber/ontologies/2020/10/ontological-engineering-project#numero_de_visitantes">
        <rdfs:domain rdf:resource="http://www.semanticweb.org/alber/ontologies/2020/10/untitled-ontology-5#Visita"/>
        <rdfs:range rdf:resource="http://www.w3.org/2001/XMLSchema#nonNegativeInteger"/>
        <rdfs:label xml:lang="en">Number of visitors</rdfs:label>
        <rdfs:label xml:lang="es">Número de visitantes</rdfs:label>
    </owl:DatatypeProperty>
    


    <!-- http://www.w3.org/2006/time#month -->

    <owl:DatatypeProperty rdf:about="http://www.w3.org/2006/time#month">
        <rdfs:domain rdf:resource="http://www.w3.org/2006/time#GeneralDateTimeDescription"/>
        <rdfs:range rdf:resource="http://www.w3.org/2001/XMLSchema#string"/>
        <rdfs:comment xml:lang="en">Month position in a calendar-clock system.

The range of this property is not specified, so can be replaced by any specific representation of a calendar month from any calendar. </rdfs:comment>
        <rdfs:comment xml:lang="es">Posición de mes en un sistema calendario-reloj.
    El rango de esta propiedad no está especificado, por tanto, se puede reemplazar por cualquier representación específica de un mes de calendario de un calendario cualquiera.</rdfs:comment>
        <rdfs:label xml:lang="es">mes</rdfs:label>
        <rdfs:label xml:lang="en">month</rdfs:label>
        <skos:definition xml:lang="en">Month position in a calendar-clock system.

The range of this property is not specified, so can be replaced by any specific representation of a calendar month from any calendar. </skos:definition>
        <skos:definition xml:lang="es">Posición de mes en un sistema calendario-reloj.
            El rango de esta propiedad no está especificado, por tanto, se puede reemplazar por cualquier representación específica de un mes de calendario de un calendario cualquiera.</skos:definition>
    </owl:DatatypeProperty>
    


    <!-- http://www.w3.org/2006/time#year -->

    <owl:DatatypeProperty rdf:about="http://www.w3.org/2006/time#year">
        <rdfs:domain rdf:resource="http://www.w3.org/2006/time#GeneralDateTimeDescription"/>
        <rdfs:range rdf:resource="http://www.w3.org/2001/XMLSchema#integer"/>
        <rdfs:comment xml:lang="es">Posición de año en un sistema calendario-reloj.

l rango de esta propiedad no está especificado, por tanto, se puede reemplazar por cualquier representación específica de un año de calendario de un calendario cualquiera.</rdfs:comment>
        <rdfs:comment xml:lang="en">Year position in a calendar-clock system.

The range of this property is not specified, so can be replaced by any specific representation of a calendar year from any calendar. </rdfs:comment>
        <rdfs:label xml:lang="en">year</rdfs:label>
    </owl:DatatypeProperty>
    


    <!-- 
    ///////////////////////////////////////////////////////////////////////////////////////
    //
    // Classes
    //
    ///////////////////////////////////////////////////////////////////////////////////////
     -->

    


    <!-- http://purl.org/NET/scovo#Dataset -->

    <owl:Class rdf:about="http://purl.org/NET/scovo#Dataset">
        <owl:equivalentClass rdf:resource="http://purl.org/linked-data/cube#DataSet"/>
    </owl:Class>
    


    <!-- http://purl.org/NET/scovo#Item -->

    <owl:Class rdf:about="http://purl.org/NET/scovo#Item">
        <owl:equivalentClass rdf:resource="http://purl.org/linked-data/cube#Observation"/>
    </owl:Class>
    


    <!-- http://purl.org/linked-data/cube#Attachable -->

    <owl:Class rdf:about="http://purl.org/linked-data/cube#Attachable"/>
    


    <!-- http://purl.org/linked-data/cube#DataSet -->

    <owl:Class rdf:about="http://purl.org/linked-data/cube#DataSet">
        <rdfs:subClassOf rdf:resource="http://purl.org/linked-data/cube#Attachable"/>
        <rdfs:comment xml:lang="en">Represents a collection of observations, possibly organized into various slices, conforming to some common dimensional structure.</rdfs:comment>
        <rdfs:isDefinedBy rdf:resource="http://purl.org/linked-data/cube"/>
        <rdfs:label xml:lang="en">Data set</rdfs:label>
    </owl:Class>
    


    <!-- http://purl.org/linked-data/cube#Observation -->

    <owl:Class rdf:about="http://purl.org/linked-data/cube#Observation">
        <rdfs:subClassOf rdf:resource="http://purl.org/linked-data/cube#Attachable"/>
        <rdfs:comment xml:lang="en">A single observation in the cube, may have one or more associated measured values</rdfs:comment>
        <rdfs:isDefinedBy rdf:resource="http://purl.org/linked-data/cube"/>
        <rdfs:label xml:lang="en">Observation</rdfs:label>
    </owl:Class>
    


    <!-- http://vocab.linkeddata.es/datosabiertos/def/urbanismo-infraestructuras/equipamiento-municipal#Equipamiento -->

    <owl:Class rdf:about="http://vocab.linkeddata.es/datosabiertos/def/urbanismo-infraestructuras/equipamiento-municipal#Equipamiento">
        <owl:equivalentClass rdf:resource="http://www.semanticweb.org/alber/ontologies/2020/10/untitled-ontology-5#Equipamiento"/>
        <rdfs:comment rdf:datatype="http://www.w3.org/2001/XMLSchema#string">Equipamientos a los que un ciudadano puede acudir pertenecientes a una administración.</rdfs:comment>
    </owl:Class>
    


    <!-- http://www.semanticweb.org/alber/ontologies/2020/10/untitled-ontology-5#Aula_de_la_naturaleza -->

    <owl:Class rdf:about="http://www.semanticweb.org/alber/ontologies/2020/10/untitled-ontology-5#Aula_de_la_naturaleza">
        <rdfs:subClassOf rdf:resource="http://www.semanticweb.org/alber/ontologies/2020/10/untitled-ontology-5#Equipamiento"/>
        <rdfs:label xml:lang="es">Aula de la naturaleza</rdfs:label>
        <rdfs:label xml:lang="en">Nature classroom</rdfs:label>
    </owl:Class>
    


    <!-- http://www.semanticweb.org/alber/ontologies/2020/10/untitled-ontology-5#CCAA -->

    <owl:Class rdf:about="http://www.semanticweb.org/alber/ontologies/2020/10/untitled-ontology-5#CCAA">
        <rdfs:subClassOf rdf:resource="http://www.semanticweb.org/alber/ontologies/2020/10/untitled-ontology-5#Lugar_Procedencia"/>
        <rdfs:subClassOf>
            <owl:Restriction>
                <owl:onProperty rdf:resource="http://www.semanticweb.org/alber/ontologies/2020/10/ontological-engineering-project#tieneParte"/>
                <owl:someValuesFrom rdf:resource="http://www.semanticweb.org/alber/ontologies/2020/10/untitled-ontology-5#Provincia"/>
            </owl:Restriction>
        </rdfs:subClassOf>
        <rdfs:subClassOf>
            <owl:Restriction>
                <owl:onProperty rdf:resource="http://www.semanticweb.org/alber/ontologies/2020/10/ontological-engineering-project#esParteDe"/>
                <owl:qualifiedCardinality rdf:datatype="http://www.w3.org/2001/XMLSchema#nonNegativeInteger">1</owl:qualifiedCardinality>
                <owl:onClass rdf:resource="http://www.semanticweb.org/alber/ontologies/2020/10/untitled-ontology-5#Pais"/>
            </owl:Restriction>
        </rdfs:subClassOf>
        <rdfs:comment xml:lang="es">Entidad territorial que, dentro del ordenamiento jurídico constitucional español, está dotada de autonomía, con instituciones y representantes propios y determinadas competencias legislativas, ejecutivas y administrativas.</rdfs:comment>
        <rdfs:comment xml:lang="en">First-level political and administrative division, created in accordance with the Spanish constitution of 1978, with the aim of guaranteeing limited autonomy of the nationalities and regions that make up Spain.</rdfs:comment>
        <rdfs:label xml:lang="en">Autonomous community</rdfs:label>
        <rdfs:label xml:lang="es">Comunidad Autónoma</rdfs:label>
    </owl:Class>
    


    <!-- http://www.semanticweb.org/alber/ontologies/2020/10/untitled-ontology-5#Camping -->

    <owl:Class rdf:about="http://www.semanticweb.org/alber/ontologies/2020/10/untitled-ontology-5#Camping">
        <rdfs:subClassOf rdf:resource="http://www.semanticweb.org/alber/ontologies/2020/10/untitled-ontology-5#Equipamiento"/>
        <rdfs:label xml:lang="en">Camping</rdfs:label>
        <rdfs:label xml:lang="es">Camping</rdfs:label>
    </owl:Class>
    


    <!-- http://www.semanticweb.org/alber/ontologies/2020/10/untitled-ontology-5#Carril_cicloturista -->

    <owl:Class rdf:about="http://www.semanticweb.org/alber/ontologies/2020/10/untitled-ontology-5#Carril_cicloturista">
        <rdfs:subClassOf rdf:resource="http://www.semanticweb.org/alber/ontologies/2020/10/untitled-ontology-5#Equipamiento"/>
        <rdfs:label xml:lang="es">Carril cicloturista</rdfs:label>
        <rdfs:label xml:lang="en">Cyclotourist lane</rdfs:label>
    </owl:Class>
    


    <!-- http://www.semanticweb.org/alber/ontologies/2020/10/untitled-ontology-5#Casa_de_artesanía -->

    <owl:Class rdf:about="http://www.semanticweb.org/alber/ontologies/2020/10/untitled-ontology-5#Casa_de_artesanía">
        <rdfs:subClassOf rdf:resource="http://www.semanticweb.org/alber/ontologies/2020/10/untitled-ontology-5#Equipamiento"/>
        <rdfs:label xml:lang="es">Casa de artesanía</rdfs:label>
        <rdfs:label xml:lang="en">Craft house</rdfs:label>
    </owl:Class>
    


    <!-- http://www.semanticweb.org/alber/ontologies/2020/10/untitled-ontology-5#Casa_rural -->

    <owl:Class rdf:about="http://www.semanticweb.org/alber/ontologies/2020/10/untitled-ontology-5#Casa_rural">
        <rdfs:subClassOf rdf:resource="http://www.semanticweb.org/alber/ontologies/2020/10/untitled-ontology-5#Equipamiento"/>
        <rdfs:label xml:lang="es">Casa rural</rdfs:label>
        <rdfs:label xml:lang="en">Rural house</rdfs:label>
    </owl:Class>
    


    <!-- http://www.semanticweb.org/alber/ontologies/2020/10/untitled-ontology-5#Centro_de_visitantes -->

    <owl:Class rdf:about="http://www.semanticweb.org/alber/ontologies/2020/10/untitled-ontology-5#Centro_de_visitantes">
        <rdfs:subClassOf rdf:resource="http://www.semanticweb.org/alber/ontologies/2020/10/untitled-ontology-5#Equipamiento"/>
        <rdfs:label xml:lang="es">Centro de visitantes</rdfs:label>
        <rdfs:label xml:lang="en">Visitors&apos; center</rdfs:label>
    </owl:Class>
    


    <!-- http://www.semanticweb.org/alber/ontologies/2020/10/untitled-ontology-5#Continente -->

    <owl:Class rdf:about="http://www.semanticweb.org/alber/ontologies/2020/10/untitled-ontology-5#Continente">
        <rdfs:subClassOf rdf:resource="http://www.semanticweb.org/alber/ontologies/2020/10/untitled-ontology-5#Lugar_Procedencia"/>
        <rdfs:subClassOf>
            <owl:Restriction>
                <owl:onProperty rdf:resource="http://www.semanticweb.org/alber/ontologies/2020/10/ontological-engineering-project#tieneParte"/>
                <owl:someValuesFrom rdf:resource="http://www.semanticweb.org/alber/ontologies/2020/10/untitled-ontology-5#Pais"/>
            </owl:Restriction>
        </rdfs:subClassOf>
        <rdfs:comment xml:lang="es">Gran extensión de Tierra que se diferencia de otras menores o sumergidas por conceptos geográficos, como son los océanos; y culturales, como la etnografía.</rdfs:comment>
        <rdfs:comment xml:lang="en">One of several very large landmasses. Generally identified by convention rather than any strict criteria, up to seven regions are commonly regarded as continents.</rdfs:comment>
        <rdfs:label xml:lang="en">Continent</rdfs:label>
        <rdfs:label xml:lang="es">Continente</rdfs:label>
    </owl:Class>
    


    <!-- http://www.semanticweb.org/alber/ontologies/2020/10/untitled-ontology-5#Ecomuseo -->

    <owl:Class rdf:about="http://www.semanticweb.org/alber/ontologies/2020/10/untitled-ontology-5#Ecomuseo">
        <rdfs:subClassOf rdf:resource="http://www.semanticweb.org/alber/ontologies/2020/10/untitled-ontology-5#Equipamiento"/>
        <rdfs:label xml:lang="es">Ecomuseo</rdfs:label>
        <rdfs:label xml:lang="en">Ecomuseum</rdfs:label>
    </owl:Class>
    


    <!-- http://www.semanticweb.org/alber/ontologies/2020/10/untitled-ontology-5#Equipamiento -->

    <owl:Class rdf:about="http://www.semanticweb.org/alber/ontologies/2020/10/untitled-ontology-5#Equipamiento">
        <rdfs:subClassOf>
            <owl:Restriction>
                <owl:onProperty rdf:resource="http://www.semanticweb.org/alber/ontologies/2020/10/ontological-engineering-project#tieneVisita"/>
                <owl:someValuesFrom rdf:resource="http://www.semanticweb.org/alber/ontologies/2020/10/untitled-ontology-5#Visita"/>
            </owl:Restriction>
        </rdfs:subClassOf>
        <rdfs:subClassOf>
            <owl:Restriction>
                <owl:onProperty rdf:resource="http://www.semanticweb.org/alber/ontologies/2020/10/ontological-engineering-project#esEquipamientoDe"/>
                <owl:qualifiedCardinality rdf:datatype="http://www.w3.org/2001/XMLSchema#nonNegativeInteger">1</owl:qualifiedCardinality>
                <owl:onClass rdf:resource="http://www.semanticweb.org/alber/ontologies/2020/10/untitled-ontology-5#Espacio_Natural"/>
            </owl:Restriction>
        </rdfs:subClassOf>
        <rdfs:comment xml:lang="es">Equipamientos a los que un ciudadano puede acudir pertenecientes a un espacio natural</rdfs:comment>
        <rdfs:comment xml:lang="en">Equipments to which citizens can go that belong to a natural space</rdfs:comment>
        <rdfs:label xml:lang="es">Equipamiento</rdfs:label>
        <rdfs:label xml:lang="en">Equipment</rdfs:label>
    </owl:Class>
    


    <!-- http://www.semanticweb.org/alber/ontologies/2020/10/untitled-ontology-5#Espacio_Natural -->

    <owl:Class rdf:about="http://www.semanticweb.org/alber/ontologies/2020/10/untitled-ontology-5#Espacio_Natural">
        <rdfs:subClassOf>
            <owl:Restriction>
                <owl:onProperty rdf:resource="http://www.semanticweb.org/alber/ontologies/2020/10/ontological-engineering-project#tieneEquipamiento"/>
                <owl:someValuesFrom rdf:resource="http://www.semanticweb.org/alber/ontologies/2020/10/untitled-ontology-5#Equipamiento"/>
            </owl:Restriction>
        </rdfs:subClassOf>
        <rdfs:subClassOf>
            <owl:Restriction>
                <owl:onProperty rdf:resource="http://www.semanticweb.org/alber/ontologies/2020/10/ontological-engineering-project#esEspacioNaturalDe"/>
                <owl:qualifiedCardinality rdf:datatype="http://www.w3.org/2001/XMLSchema#nonNegativeInteger">1</owl:qualifiedCardinality>
                <owl:onClass rdf:resource="http://www.semanticweb.org/alber/ontologies/2020/10/untitled-ontology-5#Provincia"/>
            </owl:Restriction>
        </rdfs:subClassOf>
        <rdfs:comment xml:lang="en">Part of the territoty not modified by humans and officially recognized as a protected natural space</rdfs:comment>
        <rdfs:comment xml:lang="es">Parte del territorio no modificada por el ser humano recogida oficialmente como espacio natural protegido</rdfs:comment>
        <rdfs:label xml:lang="es">Espacio natural</rdfs:label>
        <rdfs:label xml:lang="en">Natural space</rdfs:label>
    </owl:Class>
    


    <!-- http://www.semanticweb.org/alber/ontologies/2020/10/untitled-ontology-5#Hotel_de_montaña -->

    <owl:Class rdf:about="http://www.semanticweb.org/alber/ontologies/2020/10/untitled-ontology-5#Hotel_de_montaña">
        <rdfs:subClassOf rdf:resource="http://www.semanticweb.org/alber/ontologies/2020/10/untitled-ontology-5#Equipamiento"/>
        <rdfs:label xml:lang="es">Hotel de montaña</rdfs:label>
        <rdfs:label xml:lang="en">Mountain hotel</rdfs:label>
    </owl:Class>
    


    <!-- http://www.semanticweb.org/alber/ontologies/2020/10/untitled-ontology-5#Jardín_botánico -->

    <owl:Class rdf:about="http://www.semanticweb.org/alber/ontologies/2020/10/untitled-ontology-5#Jardín_botánico">
        <rdfs:subClassOf rdf:resource="http://www.semanticweb.org/alber/ontologies/2020/10/untitled-ontology-5#Equipamiento"/>
        <rdfs:label xml:lang="en">Botanic garden</rdfs:label>
        <rdfs:label xml:lang="es">Jardín botánico</rdfs:label>
    </owl:Class>
    


    <!-- http://www.semanticweb.org/alber/ontologies/2020/10/untitled-ontology-5#Kiosko_bar_restaurante -->

    <owl:Class rdf:about="http://www.semanticweb.org/alber/ontologies/2020/10/untitled-ontology-5#Kiosko_bar_restaurante">
        <rdfs:subClassOf rdf:resource="http://www.semanticweb.org/alber/ontologies/2020/10/untitled-ontology-5#Equipamiento"/>
        <rdfs:label xml:lang="en">Bar-restaurant</rdfs:label>
        <rdfs:label xml:lang="es">Kioso-bar-restaurante</rdfs:label>
    </owl:Class>
    


    <!-- http://www.semanticweb.org/alber/ontologies/2020/10/untitled-ontology-5#Lugar_Procedencia -->

    <owl:Class rdf:about="http://www.semanticweb.org/alber/ontologies/2020/10/untitled-ontology-5#Lugar_Procedencia">
        <rdfs:comment xml:lang="es">Lugar físico de donde procede un grupo de visitantes</rdfs:comment>
        <rdfs:comment xml:lang="en">Physical place where a group of visitors comes from</rdfs:comment>
        <rdfs:label xml:lang="es">Lugar de procedencia</rdfs:label>
        <rdfs:label xml:lang="en">Place of origin</rdfs:label>
    </owl:Class>
    


    <!-- http://www.semanticweb.org/alber/ontologies/2020/10/untitled-ontology-5#Mirador -->

    <owl:Class rdf:about="http://www.semanticweb.org/alber/ontologies/2020/10/untitled-ontology-5#Mirador">
        <rdfs:subClassOf rdf:resource="http://www.semanticweb.org/alber/ontologies/2020/10/untitled-ontology-5#Equipamiento"/>
        <rdfs:label xml:lang="es">Mirador</rdfs:label>
        <rdfs:label xml:lang="en">Viewpoint</rdfs:label>
    </owl:Class>
    


    <!-- http://www.semanticweb.org/alber/ontologies/2020/10/untitled-ontology-5#Observatorio -->

    <owl:Class rdf:about="http://www.semanticweb.org/alber/ontologies/2020/10/untitled-ontology-5#Observatorio">
        <rdfs:subClassOf rdf:resource="http://www.semanticweb.org/alber/ontologies/2020/10/untitled-ontology-5#Equipamiento"/>
        <rdfs:label xml:lang="es">Observatorio</rdfs:label>
        <rdfs:label xml:lang="en">Observatory</rdfs:label>
    </owl:Class>
    


    <!-- http://www.semanticweb.org/alber/ontologies/2020/10/untitled-ontology-5#Observatorio_de_uso_científico -->

    <owl:Class rdf:about="http://www.semanticweb.org/alber/ontologies/2020/10/untitled-ontology-5#Observatorio_de_uso_científico">
        <rdfs:subClassOf rdf:resource="http://www.semanticweb.org/alber/ontologies/2020/10/untitled-ontology-5#Equipamiento"/>
        <rdfs:label xml:lang="es">Observatorio de uso científico</rdfs:label>
        <rdfs:label xml:lang="en">Scientific observatory</rdfs:label>
    </owl:Class>
    


    <!-- http://www.semanticweb.org/alber/ontologies/2020/10/untitled-ontology-5#Pais -->

    <owl:Class rdf:about="http://www.semanticweb.org/alber/ontologies/2020/10/untitled-ontology-5#Pais">
        <rdfs:subClassOf rdf:resource="http://www.semanticweb.org/alber/ontologies/2020/10/untitled-ontology-5#Lugar_Procedencia"/>
        <rdfs:subClassOf>
            <owl:Restriction>
                <owl:onProperty rdf:resource="http://www.semanticweb.org/alber/ontologies/2020/10/ontological-engineering-project#tieneParte"/>
                <owl:someValuesFrom rdf:resource="http://www.semanticweb.org/alber/ontologies/2020/10/untitled-ontology-5#CCAA"/>
            </owl:Restriction>
        </rdfs:subClassOf>
        <rdfs:subClassOf>
            <owl:Restriction>
                <owl:onProperty rdf:resource="http://www.semanticweb.org/alber/ontologies/2020/10/ontological-engineering-project#esParteDe"/>
                <owl:qualifiedCardinality rdf:datatype="http://www.w3.org/2001/XMLSchema#nonNegativeInteger">1</owl:qualifiedCardinality>
                <owl:onClass rdf:resource="http://www.semanticweb.org/alber/ontologies/2020/10/untitled-ontology-5#Continente"/>
            </owl:Restriction>
        </rdfs:subClassOf>
        <rdfs:comment xml:lang="es">Territorio con características geográficas y culturales propias, que constituye un Estado soberano o una entidad política dentro de un Estado.</rdfs:comment>
        <rdfs:comment xml:lang="en">Territory with its own geographical and cultural characteristics, which constitutes a sovereign State or a political entity within a State.</rdfs:comment>
        <rdfs:label xml:lang="en">Country</rdfs:label>
        <rdfs:label xml:lang="es">País</rdfs:label>
    </owl:Class>
    


    <!-- http://www.semanticweb.org/alber/ontologies/2020/10/untitled-ontology-5#Parque_de_fauna_silvestre -->

    <owl:Class rdf:about="http://www.semanticweb.org/alber/ontologies/2020/10/untitled-ontology-5#Parque_de_fauna_silvestre">
        <rdfs:subClassOf rdf:resource="http://www.semanticweb.org/alber/ontologies/2020/10/untitled-ontology-5#Equipamiento"/>
        <rdfs:label xml:lang="es">Parque de fauna silvestre</rdfs:label>
        <rdfs:label xml:lang="en">Wildlife park</rdfs:label>
    </owl:Class>
    


    <!-- http://www.semanticweb.org/alber/ontologies/2020/10/untitled-ontology-5#Provincia -->

    <owl:Class rdf:about="http://www.semanticweb.org/alber/ontologies/2020/10/untitled-ontology-5#Provincia">
        <rdfs:subClassOf>
            <owl:Restriction>
                <owl:onProperty rdf:resource="http://www.semanticweb.org/alber/ontologies/2020/10/ontological-engineering-project#tieneEspacioNatural"/>
                <owl:someValuesFrom rdf:resource="http://www.semanticweb.org/alber/ontologies/2020/10/untitled-ontology-5#Espacio_Natural"/>
            </owl:Restriction>
        </rdfs:subClassOf>
        <rdfs:subClassOf>
            <owl:Restriction>
                <owl:onProperty rdf:resource="http://www.semanticweb.org/alber/ontologies/2020/10/ontological-engineering-project#esParteDe"/>
                <owl:qualifiedCardinality rdf:datatype="http://www.w3.org/2001/XMLSchema#nonNegativeInteger">1</owl:qualifiedCardinality>
                <owl:onClass rdf:resource="http://www.semanticweb.org/alber/ontologies/2020/10/untitled-ontology-5#CCAA"/>
            </owl:Restriction>
        </rdfs:subClassOf>
        <rdfs:comment xml:lang="es">Entidad subnacional del Estado perteneciente a una Comunidad Autónoma.</rdfs:comment>
        <rdfs:comment xml:lang="en">Subnational entity of the State.</rdfs:comment>
        <rdfs:label xml:lang="en">Province</rdfs:label>
        <rdfs:label xml:lang="es">Provincia</rdfs:label>
    </owl:Class>
    


    <!-- http://www.semanticweb.org/alber/ontologies/2020/10/untitled-ontology-5#Punto_de_información -->

    <owl:Class rdf:about="http://www.semanticweb.org/alber/ontologies/2020/10/untitled-ontology-5#Punto_de_información">
        <rdfs:subClassOf rdf:resource="http://www.semanticweb.org/alber/ontologies/2020/10/untitled-ontology-5#Equipamiento"/>
        <rdfs:label xml:lang="en">Point of information</rdfs:label>
        <rdfs:label xml:lang="es">Punto de información</rdfs:label>
    </owl:Class>
    


    <!-- http://www.semanticweb.org/alber/ontologies/2020/10/untitled-ontology-5#Refugio -->

    <owl:Class rdf:about="http://www.semanticweb.org/alber/ontologies/2020/10/untitled-ontology-5#Refugio">
        <rdfs:subClassOf rdf:resource="http://www.semanticweb.org/alber/ontologies/2020/10/untitled-ontology-5#Equipamiento"/>
        <rdfs:label xml:lang="es">Refugio</rdfs:label>
        <rdfs:label xml:lang="en">Shelter</rdfs:label>
    </owl:Class>
    


    <!-- http://www.semanticweb.org/alber/ontologies/2020/10/untitled-ontology-5#Refugio-vivac -->

    <owl:Class rdf:about="http://www.semanticweb.org/alber/ontologies/2020/10/untitled-ontology-5#Refugio-vivac">
        <rdfs:subClassOf rdf:resource="http://www.semanticweb.org/alber/ontologies/2020/10/untitled-ontology-5#Equipamiento"/>
        <rdfs:label xml:lang="es">Refugio-vivac</rdfs:label>
        <rdfs:label xml:lang="en">Shelter-bivouac</rdfs:label>
    </owl:Class>
    


    <!-- http://www.semanticweb.org/alber/ontologies/2020/10/untitled-ontology-5#Ruta_cicloturística -->

    <owl:Class rdf:about="http://www.semanticweb.org/alber/ontologies/2020/10/untitled-ontology-5#Ruta_cicloturística">
        <rdfs:subClassOf rdf:resource="http://www.semanticweb.org/alber/ontologies/2020/10/untitled-ontology-5#Equipamiento"/>
        <rdfs:label xml:lang="en">Cycle tourism route</rdfs:label>
        <rdfs:label xml:lang="es">Ruta cicloturística</rdfs:label>
    </owl:Class>
    


    <!-- http://www.semanticweb.org/alber/ontologies/2020/10/untitled-ontology-5#Sendero_señalizado -->

    <owl:Class rdf:about="http://www.semanticweb.org/alber/ontologies/2020/10/untitled-ontology-5#Sendero_señalizado">
        <rdfs:subClassOf rdf:resource="http://www.semanticweb.org/alber/ontologies/2020/10/untitled-ontology-5#Equipamiento"/>
        <rdfs:label xml:lang="es">Sendero señalizado</rdfs:label>
        <rdfs:label xml:lang="en">Signposted trail</rdfs:label>
    </owl:Class>
    


    <!-- http://www.semanticweb.org/alber/ontologies/2020/10/untitled-ontology-5#Visita -->

    <owl:Class rdf:about="http://www.semanticweb.org/alber/ontologies/2020/10/untitled-ontology-5#Visita">
        <rdfs:subClassOf rdf:resource="http://purl.org/linked-data/cube#Observation"/>
        <rdfs:subClassOf>
            <owl:Restriction>
                <owl:onProperty rdf:resource="http://www.semanticweb.org/alber/ontologies/2020/10/ontological-engineering-project#enIntervaloDeTiempo"/>
                <owl:qualifiedCardinality rdf:datatype="http://www.w3.org/2001/XMLSchema#nonNegativeInteger">1</owl:qualifiedCardinality>
                <owl:onClass rdf:resource="http://www.w3.org/2006/time#DateTimeInterval"/>
            </owl:Restriction>
        </rdfs:subClassOf>
        <rdfs:subClassOf>
            <owl:Restriction>
                <owl:onProperty rdf:resource="http://www.semanticweb.org/alber/ontologies/2020/10/ontological-engineering-project#visitaAlEquipamiento"/>
                <owl:qualifiedCardinality rdf:datatype="http://www.w3.org/2001/XMLSchema#nonNegativeInteger">1</owl:qualifiedCardinality>
                <owl:onClass rdf:resource="http://www.semanticweb.org/alber/ontologies/2020/10/untitled-ontology-5#Equipamiento"/>
            </owl:Restriction>
        </rdfs:subClassOf>
        <rdfs:subClassOf>
            <owl:Restriction>
                <owl:onProperty rdf:resource="http://www.semanticweb.org/alber/ontologies/2020/10/ontological-engineering-project#tieneProcedencia"/>
                <owl:maxQualifiedCardinality rdf:datatype="http://www.w3.org/2001/XMLSchema#nonNegativeInteger">1</owl:maxQualifiedCardinality>
                <owl:onClass rdf:resource="http://www.semanticweb.org/alber/ontologies/2020/10/untitled-ontology-5#Lugar_Procedencia"/>
            </owl:Restriction>
        </rdfs:subClassOf>
        <rdfs:comment xml:lang="en">Measure of the number of visitors that have visited an equipment</rdfs:comment>
        <rdfs:comment xml:lang="es">Medida del número de visitantes que han ido a un equipamiento</rdfs:comment>
        <rdfs:label xml:lang="en">Visit</rdfs:label>
        <rdfs:label xml:lang="es">Visita</rdfs:label>
    </owl:Class>
    


    <!-- http://www.semanticweb.org/alber/ontologies/2020/10/untitled-ontology-5#Zona_de_acampada_controlada -->

    <owl:Class rdf:about="http://www.semanticweb.org/alber/ontologies/2020/10/untitled-ontology-5#Zona_de_acampada_controlada">
        <rdfs:subClassOf rdf:resource="http://www.semanticweb.org/alber/ontologies/2020/10/untitled-ontology-5#Equipamiento"/>
        <rdfs:label xml:lang="en">Controlled camping area</rdfs:label>
        <rdfs:label xml:lang="es">Zona de acampada controlada</rdfs:label>
    </owl:Class>
    


    <!-- http://www.semanticweb.org/alber/ontologies/2020/10/untitled-ontology-5#Área_de_acampada -->

    <owl:Class rdf:about="http://www.semanticweb.org/alber/ontologies/2020/10/untitled-ontology-5#Área_de_acampada">
        <rdfs:subClassOf rdf:resource="http://www.semanticweb.org/alber/ontologies/2020/10/untitled-ontology-5#Equipamiento"/>
        <rdfs:label xml:lang="en">Camping area</rdfs:label>
        <rdfs:label xml:lang="es">Área de acampada</rdfs:label>
    </owl:Class>
    


    <!-- http://www.semanticweb.org/alber/ontologies/2020/10/untitled-ontology-5#Área_recreativa -->

    <owl:Class rdf:about="http://www.semanticweb.org/alber/ontologies/2020/10/untitled-ontology-5#Área_recreativa">
        <rdfs:subClassOf rdf:resource="http://www.semanticweb.org/alber/ontologies/2020/10/untitled-ontology-5#Equipamiento"/>
        <rdfs:label xml:lang="en">Recreational area</rdfs:label>
        <rdfs:label xml:lang="es">Área recreativa</rdfs:label>
    </owl:Class>
    


    <!-- http://www.w3.org/2006/time#DateTimeInterval -->

    <owl:Class rdf:about="http://www.w3.org/2006/time#DateTimeInterval">
        <rdfs:subClassOf rdf:resource="http://www.w3.org/2006/time#ProperInterval"/>
        <rdfs:subClassOf>
            <owl:Restriction>
                <owl:onProperty rdf:resource="http://www.semanticweb.org/alber/ontologies/2020/10/ontological-engineering-project#deVisita"/>
                <owl:someValuesFrom rdf:resource="http://www.semanticweb.org/alber/ontologies/2020/10/untitled-ontology-5#Visita"/>
            </owl:Restriction>
        </rdfs:subClassOf>
        <rdfs:comment xml:lang="es">&apos;intervalo de fecha-hora&apos; es una subclase de &apos;intervalo propio&apos;, definida utilizando el multi-elemento &apos;descripción de fecha-hora&apos;.</rdfs:comment>
        <rdfs:comment xml:lang="en">DateTimeInterval is a subclass of ProperInterval, defined using the multi-element DateTimeDescription.</rdfs:comment>
        <rdfs:label xml:lang="en">Date-time interval</rdfs:label>
        <rdfs:label xml:lang="es">intervalo de fecha-hora</rdfs:label>
        <skos:definition xml:lang="es">&apos;intervalo de fecha-hora&apos; es una subclase de &apos;intervalo propio&apos;, definida utilizando el multi-elemento &apos;descripción de fecha-hora&apos;.</skos:definition>
        <skos:definition xml:lang="en">DateTimeInterval is a subclass of ProperInterval, defined using the multi-element DateTimeDescription.</skos:definition>
        <skos:note xml:lang="es">&apos;intervalo de fecha-hora&apos; se puede utilizar sólo para un intervalo cuyos límites coinciden con un elemento de fecha-hora alineados con el calendario y la zona horaria indicados. Por ejemplo, aunque ambos tienen una duración de un día, el intervalo de 24 horas que empieza en la media noche del comienzo del 8 mayo en Europa Central se puede expresar como un &apos;intervalo de fecha-hora&apos;, el intervalo de 24 horas que empieza a las 1:30pm no.</skos:note>
        <skos:note xml:lang="en">:DateTimeInterval can only be used for an interval whose limits coincide with a date-time element aligned to the calendar and timezone indicated. For example, while both have a duration of one day, the 24-hour interval beginning at midnight at the beginning of 8 May in Central Europe can be expressed as a :DateTimeInterval, but the 24-hour interval starting at 1:30pm cannot.</skos:note>
    </owl:Class>
    


    <!-- http://www.w3.org/2006/time#GeneralDateTimeDescription -->

    <owl:Class rdf:about="http://www.w3.org/2006/time#GeneralDateTimeDescription"/>
    


    <!-- http://www.w3.org/2006/time#ProperInterval -->

    <owl:Class rdf:about="http://www.w3.org/2006/time#ProperInterval"/>
    


    <!-- 
    ///////////////////////////////////////////////////////////////////////////////////////
    //
    // Individuals
    //
    ///////////////////////////////////////////////////////////////////////////////////////
     -->

    


    <!-- http://www.semanticweb.org/alber/ontologies/2020/10/ontological-engineering-project#Almería -->

    <owl:NamedIndividual rdf:about="http://www.semanticweb.org/alber/ontologies/2020/10/ontological-engineering-project#Almería">
        <rdf:type rdf:resource="http://www.semanticweb.org/alber/ontologies/2020/10/untitled-ontology-5#Provincia"/>
        <ontological-engineering-project:esParteDe rdf:resource="http://www.semanticweb.org/alber/ontologies/2020/10/ontological-engineering-project#Andalucía"/>
        <ontological-engineering-project:tieneEspacioNatural rdf:resource="http://www.semanticweb.org/alber/ontologies/2020/10/ontological-engineering-project#Parque_Natural_Sierra_Nevada"/>
    </owl:NamedIndividual>
    


    <!-- http://www.semanticweb.org/alber/ontologies/2020/10/ontological-engineering-project#Andalucía -->

    <owl:NamedIndividual rdf:about="http://www.semanticweb.org/alber/ontologies/2020/10/ontological-engineering-project#Andalucía">
        <rdf:type rdf:resource="http://www.semanticweb.org/alber/ontologies/2020/10/untitled-ontology-5#CCAA"/>
        <ontological-engineering-project:tieneParte rdf:resource="http://www.semanticweb.org/alber/ontologies/2020/10/ontological-engineering-project#Almería"/>
    </owl:NamedIndividual>
    


    <!-- http://www.semanticweb.org/alber/ontologies/2020/10/ontological-engineering-project#Laujar_de_Andarax -->

    <owl:NamedIndividual rdf:about="http://www.semanticweb.org/alber/ontologies/2020/10/ontological-engineering-project#Laujar_de_Andarax">
        <rdf:type rdf:resource="http://www.semanticweb.org/alber/ontologies/2020/10/untitled-ontology-5#Centro_de_visitantes"/>
        <ontological-engineering-project:esEquipamientoDe rdf:resource="http://www.semanticweb.org/alber/ontologies/2020/10/ontological-engineering-project#Parque_Natural_Sierra_Nevada"/>
        <ontological-engineering-project:tieneVisita rdf:resource="http://www.semanticweb.org/alber/ontologies/2020/10/ontological-engineering-project#Visita1"/>
    </owl:NamedIndividual>
    


    <!-- http://www.semanticweb.org/alber/ontologies/2020/10/ontological-engineering-project#Parque_Natural_Sierra_Nevada -->

    <owl:NamedIndividual rdf:about="http://www.semanticweb.org/alber/ontologies/2020/10/ontological-engineering-project#Parque_Natural_Sierra_Nevada">
        <rdf:type rdf:resource="http://www.semanticweb.org/alber/ontologies/2020/10/untitled-ontology-5#Espacio_Natural"/>
        <ontological-engineering-project:esEspacioNaturalDe rdf:resource="http://www.semanticweb.org/alber/ontologies/2020/10/ontological-engineering-project#Almería"/>
        <ontological-engineering-project:tieneEquipamiento rdf:resource="http://www.semanticweb.org/alber/ontologies/2020/10/ontological-engineering-project#Laujar_de_Andarax"/>
    </owl:NamedIndividual>
    


    <!-- http://www.semanticweb.org/alber/ontologies/2020/10/ontological-engineering-project#Visita1 -->

    <owl:NamedIndividual rdf:about="http://www.semanticweb.org/alber/ontologies/2020/10/ontological-engineering-project#Visita1">
        <rdf:type rdf:resource="http://www.semanticweb.org/alber/ontologies/2020/10/untitled-ontology-5#Visita"/>
        <ontological-engineering-project:enIntervaloDeTiempo rdf:resource="http://www.semanticweb.org/alber/ontologies/2020/10/ontological-engineering-project#2018"/>
        <ontological-engineering-project:tieneProcedencia rdf:resource="http://www.semanticweb.org/alber/ontologies/2020/10/ontological-engineering-project#Andalucía"/>
        <ontological-engineering-project:visitaAlEquipamiento rdf:resource="http://www.semanticweb.org/alber/ontologies/2020/10/ontological-engineering-project#Laujar_de_Andarax"/>
        <ontological-engineering-project:numero_de_visitantes rdf:datatype="http://www.w3.org/2001/XMLSchema#integer">1919</ontological-engineering-project:numero_de_visitantes>
    </owl:NamedIndividual>
    


    <!-- http://www.semanticweb.org/alber/ontologies/2020/10/ontological-engineering-project#dataset1 -->

    <owl:NamedIndividual rdf:about="http://www.semanticweb.org/alber/ontologies/2020/10/ontological-engineering-project#dataset1">
        <rdf:type rdf:resource="http://purl.org/linked-data/cube#DataSet"/>
        <cube:dataSet rdf:resource="http://www.semanticweb.org/alber/ontologies/2020/10/ontological-engineering-project#dataset1"/>
    </owl:NamedIndividual>
    


    <!-- http://www.semanticweb.org/alber/ontologies/2020/10/ontological-engineering-project#2018 -->

    <owl:NamedIndividual rdf:about="http://www.semanticweb.org/alber/ontologies/2020/10/ontological-engineering-project#2018">
        <rdf:type rdf:resource="http://www.w3.org/2006/time#DateTimeInterval"/>
        <ontological-engineering-project:deVisita rdf:resource="http://www.semanticweb.org/alber/ontologies/2020/10/ontological-engineering-project#Visita1"/>
        <time:year rdf:datatype="http://www.w3.org/2001/XMLSchema#integer">2018</time:year>
    </owl:NamedIndividual>
    


    <!-- 
    ///////////////////////////////////////////////////////////////////////////////////////
    //
    // General axioms
    //
    ///////////////////////////////////////////////////////////////////////////////////////
     -->

    <rdf:Description>
        <rdf:type rdf:resource="http://www.w3.org/2002/07/owl#AllDisjointClasses"/>
        <owl:members rdf:parseType="Collection">
            <rdf:Description rdf:about="http://www.semanticweb.org/alber/ontologies/2020/10/untitled-ontology-5#Aula_de_la_naturaleza"/>
            <rdf:Description rdf:about="http://www.semanticweb.org/alber/ontologies/2020/10/untitled-ontology-5#Camping"/>
            <rdf:Description rdf:about="http://www.semanticweb.org/alber/ontologies/2020/10/untitled-ontology-5#Carril_cicloturista"/>
            <rdf:Description rdf:about="http://www.semanticweb.org/alber/ontologies/2020/10/untitled-ontology-5#Casa_de_artesanía"/>
            <rdf:Description rdf:about="http://www.semanticweb.org/alber/ontologies/2020/10/untitled-ontology-5#Casa_rural"/>
            <rdf:Description rdf:about="http://www.semanticweb.org/alber/ontologies/2020/10/untitled-ontology-5#Centro_de_visitantes"/>
            <rdf:Description rdf:about="http://www.semanticweb.org/alber/ontologies/2020/10/untitled-ontology-5#Ecomuseo"/>
            <rdf:Description rdf:about="http://www.semanticweb.org/alber/ontologies/2020/10/untitled-ontology-5#Hotel_de_montaña"/>
            <rdf:Description rdf:about="http://www.semanticweb.org/alber/ontologies/2020/10/untitled-ontology-5#Jardín_botánico"/>
            <rdf:Description rdf:about="http://www.semanticweb.org/alber/ontologies/2020/10/untitled-ontology-5#Kiosko_bar_restaurante"/>
            <rdf:Description rdf:about="http://www.semanticweb.org/alber/ontologies/2020/10/untitled-ontology-5#Mirador"/>
            <rdf:Description rdf:about="http://www.semanticweb.org/alber/ontologies/2020/10/untitled-ontology-5#Observatorio"/>
            <rdf:Description rdf:about="http://www.semanticweb.org/alber/ontologies/2020/10/untitled-ontology-5#Observatorio_de_uso_científico"/>
            <rdf:Description rdf:about="http://www.semanticweb.org/alber/ontologies/2020/10/untitled-ontology-5#Parque_de_fauna_silvestre"/>
            <rdf:Description rdf:about="http://www.semanticweb.org/alber/ontologies/2020/10/untitled-ontology-5#Punto_de_información"/>
            <rdf:Description rdf:about="http://www.semanticweb.org/alber/ontologies/2020/10/untitled-ontology-5#Refugio"/>
            <rdf:Description rdf:about="http://www.semanticweb.org/alber/ontologies/2020/10/untitled-ontology-5#Refugio-vivac"/>
            <rdf:Description rdf:about="http://www.semanticweb.org/alber/ontologies/2020/10/untitled-ontology-5#Ruta_cicloturística"/>
            <rdf:Description rdf:about="http://www.semanticweb.org/alber/ontologies/2020/10/untitled-ontology-5#Sendero_señalizado"/>
            <rdf:Description rdf:about="http://www.semanticweb.org/alber/ontologies/2020/10/untitled-ontology-5#Zona_de_acampada_controlada"/>
            <rdf:Description rdf:about="http://www.semanticweb.org/alber/ontologies/2020/10/untitled-ontology-5#Área_de_acampada"/>
            <rdf:Description rdf:about="http://www.semanticweb.org/alber/ontologies/2020/10/untitled-ontology-5#Área_recreativa"/>
        </owl:members>
    </rdf:Description>
</rdf:RDF>



<!-- Generated by the OWL API (version 4.5.9.2019-02-01T07:24:44Z) https://github.com/owlcs/owlapi -->

